tweetnacl20140427/verif_crypto_stream.v
@@ -13,32 +13,7 @@ Require Import tweetnacl20140427.Snuffle.
 Require Import tweetnacl20140427.spec_salsa. Opaque Snuffle.Snuffle.
 Require Import tweetnacl20140427.verif_crypto_stream_salsa20_xor.
 
-(*TODO: support the following part of the tetxual spec:
-      m and c can point to the same address (in-place encryption/decryption). 
-     If they don't, the regions should not overlap.*)
-Definition f_crypto_stream_salsa20_tweet_spec := 
-  DECLARE _crypto_stream_salsa20_tweet
-   WITH c : val, k:val, nonce:val, d:int64,
-        Nonce : SixteenByte, K: SixteenByte * SixteenByte,
-        (*mCont: list byte, *) SV:val
-   PRE [ _c OF tptr tuchar, (*_m OF tptr tuchar,*) _d OF tulong,
-         _n OF tptr tuchar, _k OF tptr tuchar]
-      PROP ((*Zlength mCont = Int64.unsigned b*))
-      LOCAL (temp _c c; (*temp _m m;*) temp _d (Vlong d);
-             temp _n nonce; temp _k k; gvar _sigma SV)
-      SEP ( SByte Nonce nonce;
-            data_at_ Tsh (Tarray tuchar (Int64.unsigned d) noattr) c;
-            ThirtyTwoByte K k;
-            Sigma_vector SV
-            (*data_at Tsh (tarray tuchar (Zlength mCont)) (Bl2VL mCont) m*))
-  POST [ tint ] 
-       PROP ()
-       LOCAL (temp ret_temp (Vint (Int.repr 0)))
-       SEP (Sigma_vector SV; 
-            ThirtyTwoByte K k;
-            crypto_stream_xor_postsep d Nonce K (list_repeat (Z.to_nat (Int64.unsigned d)) Byte.zero) (Int64.unsigned d) nonce c nullval). 
-
-Lemma crypto_stream_salsa20_tweet_ok: semax_body SalsaVarSpecs (crypto_stream_salsa20_xor_spec::SalsaFunSpecs)
+Lemma crypto_stream_salsa20_tweet_ok: semax_body SalsaVarSpecs (*(crypto_stream_salsa20_xor_spec::*)SalsaFunSpecs
       f_crypto_stream_salsa20_tweet
       f_crypto_stream_salsa20_tweet_spec.
 Proof. 
@@ -51,35 +26,9 @@ apply Zlength_list_repeat. apply Int64.unsigned_range.
 forward.
 Qed.
 
-Definition f_crypto_stream_xsalsa20_tweet_spec := 
-  DECLARE _crypto_stream_xsalsa20_tweet
-   WITH c : val, k:val, nonce:val, d:int64,
-        Nonce : SixteenByte, Nonce2 : SixteenByte, K: SixteenByte * SixteenByte,
-        SV:val
-   PRE [ _c OF tptr tuchar,  _d OF tulong,
-         _n OF tptr tuchar, _k OF tptr tuchar]
-      PROP ()
-      LOCAL (temp _c c; (*temp _m m;*) temp _d (Vlong d);
-             temp _n nonce; temp _k k; gvar _sigma SV)
-      SEP ( SByte Nonce nonce; SByte Nonce2 (offset_val 16 nonce);
-            data_at_ Tsh (Tarray tuchar (Int64.unsigned d) noattr) c;
-            ThirtyTwoByte K k;
-            Sigma_vector SV
-            (*data_at Tsh (tarray tuchar (Zlength mCont)) (Bl2VL mCont) m*))
-  POST [ tint ] 
-       PROP ()
-       LOCAL (temp ret_temp (Vint (Int.repr 0)))
-       SEP (Sigma_vector SV; 
-            EX HSalsaRes:_, crypto_stream_xor_postsep d Nonce2 HSalsaRes
-              (list_repeat (Z.to_nat (Int64.unsigned d)) Byte.zero) (Int64.unsigned d)
-              (offset_val 16 nonce) c nullval;
-            data_at Tsh (Tarray tuchar 16 noattr) (SixteenByte2ValList Nonce) nonce;
-            ThirtyTwoByte K k).
-(*            crypto_stream_xor_postsep d Nonce K (list_repeat (Z.to_nat (Int64.unsigned d)) Byte.zero) (Int64.unsigned d) nonce c k nullval). *)
-
 (*The crypto_stream function*)
 Lemma crypto_stream_xsalsa20_tweet_ok: 
-      semax_body SalsaVarSpecs (crypto_stream_salsa20_xor_spec::f_crypto_stream_salsa20_tweet_spec::SalsaFunSpecs)
+      semax_body SalsaVarSpecs SalsaFunSpecs
       f_crypto_stream_xsalsa20_tweet
       f_crypto_stream_xsalsa20_tweet_spec.
 Proof. 
@@ -119,35 +68,10 @@ simpl. Exists s. unfold ThirtyTwoByte. entailer.
 destruct HSalsaRes as [q1 q2]. cancel.
 Qed.
 
-Definition f_crypto_stream_xsalsa20_tweet_xor_spec := 
-  DECLARE _crypto_stream_salsa20_tweet_xor
-   WITH c : val, k:val, nonce:val, m:val, d:int64, mCont: list byte,
-        Nonce : SixteenByte, Nonce2 : SixteenByte, K: SixteenByte * SixteenByte,
-        SV:val
-   PRE [ _c OF tptr tuchar, _m OF tptr tuchar,  _d OF tulong,
-         _n OF tptr tuchar, _k OF tptr tuchar]
-      PROP (Zlength mCont = Int64.unsigned d)
-      LOCAL (temp _c c; temp _m m; temp _d (Vlong d);
-             temp _n nonce; temp _k k; gvar _sigma SV)
-      SEP ( SByte Nonce nonce; SByte Nonce2 (offset_val 16 nonce);
-            data_at_ Tsh (Tarray tuchar (Int64.unsigned d) noattr) c;
-            ThirtyTwoByte K k;
-            message_at mCont m;
-            Sigma_vector SV
-            (*data_at Tsh (tarray tuchar (Zlength mCont)) (Bl2VL mCont) m*))
-  POST [ tint ] 
-       PROP ()
-       LOCAL (temp ret_temp (Vint (Int.repr 0)))
-       SEP (Sigma_vector SV; 
-            EX HSalsaRes:_, crypto_stream_xor_postsep d Nonce2 HSalsaRes
-              mCont (Int64.unsigned d)
-              (offset_val 16 nonce) c m;
-            data_at Tsh (Tarray tuchar 16 noattr) (SixteenByte2ValList Nonce) nonce;
-            ThirtyTwoByte K k).
 
 (*The crypto_stream_xor function*)
 Lemma crypto_stream_xsalsa20_tweet_xor_ok: 
-      semax_body SalsaVarSpecs (crypto_stream_salsa20_xor_spec::f_crypto_stream_salsa20_tweet_spec::SalsaFunSpecs)
+      semax_body SalsaVarSpecs SalsaFunSpecs
       f_crypto_stream_xsalsa20_tweet_xor
       f_crypto_stream_xsalsa20_tweet_xor_spec.
 Proof. 
